src/ReactorModel/Execution/Theorems/Grouped/Instantaneous.lean
@@ -1,4 +1,5 @@
-import ReactorModel.Execution.Trace
+import ReactorModel.Execution.Theorems.SkipStep
+import ReactorModel.Execution.Theorems.ExecStep
 
 open ReactorType
 
@@ -24,57 +25,72 @@ structure Closed (s₁ s₂ : State α) where
 
 notation s₁:max " ↓ᵢ| " s₂:max => Closed s₁ s₂
 
-/- Step:
+variable {s₁ s₂ : State α}
 
-variable [Proper α] {s₁ s₂ : State α} in section
+instance : Coe (s₁ ↓ₛ s₂) (Step s₁ s₂) where
+  coe := Step.skip
+
+instance : Coe (s₁ ↓ₑ s₂) (Step s₁ s₂) where
+  coe := Step.exec
+
+namespace Step
   
-theorem mem_progress_iff (e : s₁ ⇓ᵢ s₂) : rcn' ∈ s₂.progress ↔ rcn' = e.rcn ∨ rcn' ∈ s₁.progress := 
-  by cases e <;> simp [State.mem_record_progress_iff, rcn, State.exec_preserves_progress]
+def rcn : (s₁ ↓ᵢ s₂) → ID 
+  | skip e | exec e => e.rcn
 
--- Corollary of `InstStep.mem_progress_iff`.
-theorem progress_monotonic (e : s₁ ⇓ᵢ s₂) (h : rcn' ∈ s₁.progress) : rcn' ∈ s₂.progress := 
-  e.mem_progress_iff.mpr $ .inr h
+theorem allows_rcn : (e : s₁ ↓ᵢ s₂) → s₁.Allows e.rcn 
+  | skip e | exec e => e.allows_rcn
 
--- Corollary of `InstStep.mem_progress_iff`.
-theorem rcn_mem_progress : (e : s₁ ⇓ᵢ s₂) → e.rcn ∈ s₂.progress := 
-  (·.mem_progress_iff.mpr $ .inl rfl)
+theorem preserves_tag : (s₁ ↓ᵢ s₂) → s₁.tag = s₂.tag 
+  | skip e | exec e => e.preserves_tag
 
-theorem rcn_not_mem_progress (e : s₁ ⇓ᵢ s₂) : e.rcn ∉ s₁.progress := 
+theorem equiv : (s₁ ↓ᵢ s₂) → s₁.rtr ≈ s₂.rtr
+  | skip e | exec e => e.equiv
+
+theorem progress_eq : (e : s₁ ↓ᵢ s₂) → s₂.progress = s₁.progress.insert e.rcn
+  | skip e | exec e => e.progress_eq
+
+-- Corollary of `InstStep.progress_eq`.
+theorem progress_monotonic {rcn : ID} (e : s₁ ↓ᵢ s₂) (h : rcn ∈ s₁.progress) : rcn ∈ s₂.progress :=
+  e.progress_eq ▸ Set.mem_insert_of_mem _ h
+
+-- Corollary of `InstStep.progress_eq`.
+theorem rcn_mem_progress (e : s₁ ↓ᵢ s₂) : e.rcn ∈ s₂.progress :=
+  e.progress_eq ▸ Set.mem_insert _ _
+  
+theorem rcn_not_mem_progress (e : s₁ ↓ᵢ s₂) : e.rcn ∉ s₁.progress := 
   e.allows_rcn.unprocessed
 
-theorem not_closed (e : s₁ ⇓ᵢ s₂) : ¬s₁.Closed :=
+theorem not_closed (e : s₁ ↓ᵢ s₂) : ¬s₁.Closed :=
   (· ▸ e.allows_rcn.unprocessed $ e.allows_rcn.mem)
 
-theorem preserves_tag : (s₁ ⇓ᵢ s₂) → s₁.tag = s₂.tag 
-  | skip .. | exec .. => by simp [State.record_preserves_tag, State.exec_preserves_tag]
+theorem deterministic (e₁ : s ↓ᵢ s₁) (e₂ : s ↓ᵢ s₂) (h : e₁.rcn = e₂.rcn) : s₁ = s₂ := by
+  cases e₁ <;> cases e₂ <;> simp [rcn] at h
+  case skip.skip e₁ e₂ => simp [e₁.dst_eq, e₂.dst_eq, h]
+  case exec.exec e₁ e₂ => simp [e₁.dst_eq, e₂.dst_eq, h, e₁.apply.deterministic (h.symm ▸ e₂.apply)]
+  all_goals
+    have := ‹_ ↓ₛ _›.not_triggers_rcn
+    have := ‹_ ↓ₑ _›.triggers_rcn
+    simp_all
 
-theorem equiv : (s₁ ⇓ᵢ s₂) → s₁.rtr ≈ s₂.rtr
-  | skip .. => .refl _
-  | exec .. => s₁.exec_equiv _
-
-theorem deterministic (e₁ : s ⇓ᵢ s₁) (e₂ : s ⇓ᵢ s₂) (h : e₁.rcn = e₂.rcn) : s₁ = s₂ := by
-  cases e₁ <;> cases e₂
-  all_goals simp [rcn] at h; subst h; first | rfl | contradiction
-
-theorem acyclic (e : s₁ ⇓ᵢ s₂) : e.rcn ≮[s₁.rtr] e.rcn :=
+theorem acyclic (e : s₁ ↓ᵢ s₂) : e.rcn ≮[s₁.rtr] e.rcn :=
   e.allows_rcn.acyclic
 
-theorem progress_eq : (e : s₁ ⇓ᵢ s₂) → s₂.progress = s₁.progress.insert e.rcn
-  | skip .. | exec .. => by simp [State.exec_preserves_progress, State.record]; rfl
-
-theorem progress_ssubset (e : s₁ ⇓ᵢ s₂) : s₁.progress ⊂ s₂.progress := by
+theorem progress_ssubset (e : s₁ ↓ᵢ s₂) : s₁.progress ⊂ s₂.progress := by
   simp [e.progress_eq, Set.ssubset_iff_insert]
   exists e.rcn, e.allows_rcn.unprocessed
 
-theorem seq_wellordered (e₁ : s₁ ⇓ᵢ s₂) (e₂ : s₂ ⇓ᵢ s₃) : e₂.rcn ≮[s₁.rtr] e₁.rcn := by
+theorem seq_wellordered (e₁ : s₁ ↓ᵢ s₂) (e₂ : s₂ ↓ᵢ s₃) : e₂.rcn ≮[s₁.rtr] e₁.rcn := by
   by_contra d
   exact e₂.allows_rcn.unprocessed $ e₁.progress_monotonic $ e₁.allows_rcn.deps d
 
-theorem seq_rcn_ne (e₁ : s₁ ⇓ᵢ s₂) (e₂ : s₂ ⇓ᵢ s₃) : e₁.rcn ≠ e₂.rcn := by
+theorem seq_rcn_ne (e₁ : s₁ ↓ᵢ s₂) (e₂ : s₂ ↓ᵢ s₃) : e₁.rcn ≠ e₂.rcn := by
   by_contra he
   exact e₂.allows_rcn.unprocessed (he ▸ e₁.rcn_mem_progress)
 
-end
+end Step
+
+/- Step:
 
 variable [Practical α] {s₁ s₂ s₃ : State α}
 
