src/ReactorModel/Execution/Theorems/Grouped/Steps.lean
@@ -1,5 +1,6 @@
-import ReactorModel.Execution.Trace
+import ReactorModel.Execution.Basic
 import ReactorModel.Execution.Theorems.Grouped.Instantaneous
+import ReactorModel.Execution.Theorems.Nontrivial
 
 open ReactorType
 
@@ -7,17 +8,50 @@ namespace Execution.Grouped
 
 variable [Indexable α]
 
+inductive Step (s₁ s₂ : State α)
+  | inst : (s₁ ↓ᵢ| s₂) → Step s₁ s₂
+  | time : (s₁ ↓ₜ s₂) → Step s₁ s₂
+
+namespace Step
+
+variable {s₁ s₂ : State α}
+
+theorem deterministic (e₁ : Step s s₁) (e₂ : Step s s₂) : s₁ = s₂ := by
+  sorry
+
+instance : Coe (s₁ ↓ᵢ| s₂) (Step s₁ s₂) where
+  coe := inst
+
+instance : Coe (s₁ ↓ₜ s₂) (Step s₁ s₂) where
+  coe := time
+
+end Step
+
 inductive Steps : State α → State α → Type 
   | refl : Steps s s
-  | step : (s₂ ↓ₜ s₃) → (s₁ ↓ᵢ| s₂) → (Steps s₃ s₄) → Steps s₁ s₄ 
+  | step : (Step s₁ s₂) → (Steps s₂ s₃) → Steps s₁ s₃ 
 
 namespace Steps
 
-theorem tag_strictly_monotonic {s₁ : State α} (e : Steps s₁ s₂) : s₁.tag < s₂.tag := by
+theorem tag_lt {s₁ : State α} (e : Steps s₁ s₂) : s₁.tag < s₂.tag := by
   sorry
 
-theorem deterministic {s₁ s₂ : State α} (e₁ : Steps s s₁) (e₂ : Steps s s₂) 
-    (ht : s₁.tag = s₂.tag) : s₁ = s₂ := by
-  sorry
+theorem deterministic {s₁ s₂ : State α} (e₁ : Steps s s₁) (e₂ : Steps s s₂) (n : s.Nontrivial)
+    (ht : s₁.tag = s₂.tag) (hp : s₁.progress = s₂.progress) : s₁ = s₂ := by
+  induction e₁ <;> cases e₂
+  case refl.refl => rfl
+  case step.step e₁ _ hi _ e₂ e₂' => 
+    exact hi (e₁.deterministic e₂ ▸ e₂') sorry ht hp
+  all_goals cases ‹Step _ _›
+  case refl.step.time e' e =>
+    have := e.tag_lt
+    sorry -- s.tag < tl₂.tag
+  case step.refl.time e' _ e =>
+    have := e.tag_lt
+    sorry -- tl₂.tag < s.tag
+  case refl.step.inst =>
+    sorry -- s.progress ⊂ tl₂.progress 
+  case step.refl.inst =>
+    sorry -- tl₂.progress ⊂ s.progress 
 
 end Execution.Grouped.Steps
