src/ReactorModel/Execution/Theorems/Grouped/Tail.lean
@@ -1,4 +1,6 @@
-import ReactorModel.Execution.Trace
+import ReactorModel.Execution.Basic
+import ReactorModel.Execution.Theorems.Grouped.Instantaneous
+
 open ReactorType
 
 namespace Execution.Grouped
@@ -6,7 +8,16 @@ namespace Execution.Grouped
 variable [Indexable α]
 
 inductive Tail : State α → State α → Type
-  | nil  : Tail s s
-  | time : (s₁ ↓ₜ s₂) → Tail s₁ s₂
+  | none  : Tail s s
+  | some : (s₁ ↓ᵢ+ s₂) → Tail s₁ s₂
 
-end Execution.Grouped
+namespace Tail
+
+theorem preserves_tag {s₁ : State α} (e : Tail s₁ s₂) : s₁.tag = s₂.tag := by
+  sorry
+
+theorem deterministic {s₁ s₂ : State α} (e₁ : Tail s s₁) (e₂ : Tail s s₂) 
+    (hp : s₁.progress = s₂.progress) : s₁ = s₂ := by
+  sorry
+
+end Execution.Grouped.Tail
