src/ReactorModel/Execution/Theorems/SkipStep.lean
@@ -1,0 +1,24 @@
+import ReactorModel.Execution.Basic
+
+open Classical ReactorType Execution State
+
+namespace Execution.Step.Skip
+
+variable [Indexable α] {s₁ : State α}
+
+def rcn :                      (s₁ ↓ₛ s₂) → ID                   | .mk (rcn := rcn) .. => rcn
+theorem allows_rcn :       (e : s₁ ↓ₛ s₂) → Allows s₁ e.rcn      | .mk a _ => a
+theorem not_triggers_rcn : (e : s₁ ↓ₛ s₂) → ¬Triggers s₁ e.rcn   | .mk _ t => t
+theorem dst_eq :           (e : s₁ ↓ₛ s₂) → s₂ = s₁.record e.rcn | .mk .. => rfl
+
+theorem preserves_tag (e : s₁ ↓ₛ s₂) : s₁.tag = s₂.tag := by
+  simp [e.dst_eq, State.record_preserves_tag]
+
+theorem equiv (e : s₁ ↓ₛ s₂) : s₁.rtr ≈ s₂.rtr := by
+  simp [e.dst_eq, State.record_preserves_rtr]
+  exact .refl _
+
+theorem progress_eq (e : s₁ ↓ₛ s₂) : s₂.progress = s₁.progress.insert e.rcn := by 
+  simp [e.dst_eq, State.record_progress_eq]
+
+end Execution.Step.Skip
